txn-data-consistency/EP+_Reduction.thy
@@ -1,8 +1,31 @@
 section \<open>Partial order reduction\<close>
 
-theory Partial_Order_Reduction
+theory "EP+_Reduction"
   imports "EP+_TCCv" Reductions
 begin
+
+
+text \<open>Some congruence lemmas for explorative proofs\<close>
+
+lemma fun_upd1_cong: 
+  "\<lbrakk> a = b \<rbrakk> \<Longrightarrow> f(x := a) = f(x := b)"
+  by auto
+
+lemma fun_upd2_cong: 
+  "\<lbrakk> a = c; b = d \<rbrakk> \<Longrightarrow> f(x := a, y := b) = f(x := c, y := d)"
+  by auto
+
+lemma global_conf_rtxn_cls_twisted_update_cong:
+  "s\<lparr>rtxn_rts := b, cls := a\<rparr> = s\<lparr> cls := a, rtxn_rts := b\<rparr>"
+  by auto
+
+thm cl_conf.unfold_congs
+thm global_conf.unfold_congs
+
+lemma global_conf_svrs_cls_twisted_update_cong:
+  "\<lbrakk> X = X'; Y = Y'; Z = Z' \<rbrakk> \<Longrightarrow> s\<lparr>svrs := X, cls := Y, rtxn_rts := Z\<rparr> = s\<lparr>cls := Y', rtxn_rts := Z', svrs := X'\<rparr>" 
+  by auto
+
 
 \<comment> \<open>read_invoke\<close>
 lemma read_invoke_read_invoke_indep:
@@ -27,18 +50,7 @@ lemma read_invoke_write_commit_indep:
 
 lemma read_invoke_write_done_indep:
   "cl \<noteq> cl' \<Longrightarrow> left_commute tps (RInvoke cl keys) (WDone cl' kv_map')"
-  apply (auto simp add: left_commute')
-  subgoal for s w s'
-  proof -
-    assume a: "cl \<noteq> cl'" "write_done cl' kv_map' s w" "read_invoke cl keys w s'"
-    hence "(\<lambda>ka. if kv_map' ka = None then lst_map (cls (read_invoke_U cl keys s) cl') ka
-              else get_lst (svr_state (svrs (read_invoke_U cl keys s) ka)
-                     (get_wtxn (read_invoke_U cl keys s) cl'))) = 
-           (\<lambda>k. if kv_map' k = None then lst_map (cls s cl') k
-              else get_lst (svr_state (svrs s k) (get_wtxn s cl')))" by auto
-    then show ?thesis using a by (auto simp add: tps_trans_defs fun_upd_twist)
-  qed
-  done
+  by (auto simp add: left_commute' tps_trans_defs fun_upd_twist ext)
 
 lemma read_invoke_register_read_indep:
   "cl \<noteq> get_cl t' \<Longrightarrow> left_commute tps (RInvoke cl keys) (RegR k' t' i' rts')"
@@ -77,18 +89,7 @@ lemma read_write_commit_indep:
 
 lemma read_write_done_indep:
   "cl \<noteq> cl' \<Longrightarrow> left_commute tps (Read cl k v t rts rlst) (WDone cl' kv_map')"
-  apply (auto simp add: left_commute')
-  subgoal for s w s'
-  proof -
-    assume a: "cl \<noteq> cl'" "write_done cl' kv_map' s w" "read cl k v t rts rlst w s'"
-    hence "(\<lambda>ka. if kv_map' ka = None then lst_map (cls (read_U cl k v rts rlst s) cl') ka
-              else get_lst (svr_state (svrs (read_U cl k v rts rlst s) ka)
-                     (get_wtxn (read_U cl k v rts rlst s) cl'))) = 
-           (\<lambda>k. if kv_map' k = None then lst_map (cls s cl') k
-              else get_lst (svr_state (svrs s k) (get_wtxn s cl')))" by auto
-    then show ?thesis using a by (auto simp add: tps_trans_defs fun_upd_twist)
-  qed
-  done
+  by (auto simp add: left_commute' tps_trans_defs fun_upd_twist ext)
 
 lemma read_register_read_indep:
   "cl \<noteq> get_cl t' \<Longrightarrow> left_commute tps (Read cl k v t_wr rts rlst) (RegR k' t' t_wr' rts')"
@@ -124,58 +125,36 @@ lemma read_done_write_invoke_indep:
 (*
   TODO:
 *)
-term Union
-
-lemma read_done_write_commit_indep_L1:   (*  *)
-  "cl \<noteq> cl' \<Longrightarrow> 
-  get_ctx (s\<lparr>cls := (cls s)(cl' := X), 
-             wtxn_deps := (wtxn_deps s)(get_wtxn s cl' := cl_ctx (cls s cl')),
-             wtxn_cts := (wtxn_cts s) (get_wtxn s cl' \<mapsto> cts)\<rparr>) cl keys = 
-  get_ctx s cl keys"
-  apply (auto simp add: get_view_def del: equalityI)
-  apply (intro arg_cong[where f="Union"] arg_cong[where f="\<lambda>g. image g _"] ext)
-  (* DOES NOT SEEM TO HOLD, requires removal of history variable wtxn_deps? *)
-  sorry
 
 lemma read_done_write_commit_indep:
   "cl \<noteq> cl' \<Longrightarrow> left_commute tps (RDone cl kv_map sn u'') (WCommit cl' kv_map' cts' sn' u''')"
   apply (auto simp add: left_commute' read_done_def write_commit_def)
   subgoal for s
-    by (auto simp add: tps_trans_defs)
+    apply (auto simp add: tps_trans_defs)
+    sorry
 
   subgoal for s
-    by (auto simp add: tps_trans_defs)
+    apply (auto simp add: tps_trans_defs)
+    sorry
 
   subgoal for s
-    by (auto simp add: tps_trans_defs read_done_write_commit_indep_L1 fun_upd_twist)
-
+    by (auto simp add: tps_trans_defs fun_upd_twist)
   done
 
 
-
 term fun_upd
-
-lemma fun_upd1_cong: 
-  "\<lbrakk> a = b \<rbrakk> \<Longrightarrow> f(x := a) = f(x := b)"
-  by auto
-
-lemma fun_upd2_cong: 
-  "\<lbrakk> a = c; b = d \<rbrakk> \<Longrightarrow> f(x := a, y := b) = f(x := c, y := d)"
-  by auto
-
-lemma global_conf_rtxn_cls_twisted_update_cong:
-  "s\<lparr>rtxn_rts := b, cls := a\<rparr> = s\<lparr> cls := a, rtxn_rts := b\<rparr>"
-  by auto
 
 
 lemma read_done_write_done_indep:
   "cl \<noteq> cl' \<Longrightarrow> left_commute tps (RDone cl kv_map sn u'') (WDone cl' kv_map')"
   apply (auto simp add: left_commute' read_done_def write_done_def)
   subgoal for s
-    by (auto simp add: tps_trans_defs)
+    apply (auto simp add: tps_trans_defs)
+    sorry
 
   subgoal for s
-    by (auto simp add: tps_trans_defs)
+    apply (auto simp add: tps_trans_defs)
+    sorry
 
   subgoal for s
     apply (auto simp add: tps_trans_defs get_view_def global_conf_rtxn_cls_twisted_update_cong)
@@ -184,13 +163,6 @@ lemma read_done_write_done_indep:
     by (intro fun_upd2_cong cl_conf.fold_congs arg_cong[where f="(\<union>) _"], auto del: equalityI)
   done 
 
-thm cl_conf.unfold_congs
-thm global_conf.unfold_congs
-
-
-lemma global_conf_svrs_cls_twisted_update_cong:
-  "\<lbrakk> X = X'; Y = Y'; Z = Z' \<rbrakk> \<Longrightarrow> s\<lparr>svrs := X, cls := Y, rtxn_rts := Z\<rparr> = s\<lparr>cls := Y', rtxn_rts := Z', svrs := X'\<rparr>" 
-  by auto
 
 \<comment> \<open>taken from the EP+_TCCv_proof.thy\<close>
 
@@ -236,61 +208,43 @@ lemma read_done_register_read_indep:
   "cl \<noteq> get_cl t' \<Longrightarrow> left_commute tps (RDone cl kv_map sn u'') (RegR k' t' t_wr' rts')"
   apply (auto simp add: left_commute' read_done_def register_read_def)
   subgoal for s
-    by (auto simp add: tps_trans_defs)
+    apply (auto simp add: tps_trans_defs)
+    sorry
 
   subgoal for s
-    by (auto simp add: tps_trans_defs)
+    apply (auto simp add: tps_trans_defs)
+    sorry
 
   subgoal for s
-    apply (auto simp add: tps_trans_defs get_view_def)
-    apply (intro global_conf_svrs_cls_twisted_update_cong, simp)
-    apply (intro fun_upd1_cong cl_conf.fold_congs arg_cong[where f="(\<union>) _"], simp_all)
-    by (metis add_to_readerset_pres_read_at)
+    by (auto simp add: tps_trans_defs get_view_def)
   done 
 
 lemma read_done_prepare_write_indep:
   "cl \<noteq> get_cl_w t' \<Longrightarrow> left_commute tps (RDone cl kv_map sn u'') (PrepW k' t' v')"
   apply (auto simp add: left_commute' read_done_def prepare_write_def)
   subgoal for s
-    by (auto simp add: tps_trans_defs)
-
-  subgoal for s
-    by (auto simp add: tps_trans_defs)
-
-  subgoal for s
     apply (auto simp add: tps_trans_defs)
-    apply (intro global_conf_svrs_cls_twisted_update_cong, simp)
-    apply (intro fun_upd1_cong cl_conf.unfold_congs arg_cong[where f="(\<union>) _"], simp_all)
-    (* DOES NOT HOLD? (changes get_ts on server k') *)
     sorry
 
+  subgoal for s
+    by (auto simp add: tps_trans_defs)
+
+  subgoal for s
+    by (auto simp add: tps_trans_defs)
   done 
 
 lemma read_done_commit_write_indep:
   "cl \<noteq> get_cl_w t \<Longrightarrow> left_commute tps (RDone cl kv_map sn u'') (CommitW k' t' v' cts')"
   apply (auto simp add: left_commute' read_done_def commit_write_def)
   subgoal for s
-    by (auto simp add: tps_trans_defs)
-
-  subgoal for s
-    by (auto simp add: tps_trans_defs)
-
-  subgoal for s
     apply (auto simp add: tps_trans_defs)
-    subgoal for kv_map' ts y 
-      apply (intro global_conf_svrs_cls_twisted_update_cong, simp)
-      apply (intro fun_upd1_cong cl_conf.unfold_congs arg_cong[where f="(\<union>) _"], simp_all)
-      (* DOES NOT HOLD? (changes get_ts on server side) *)
-      sorry
+    sorry
 
-    subgoal for kv_map' ts y x
-      thm contrapos_np
-      apply (erule contrapos_np[where Q="(_ :: 'v global_conf)= _"])
-      apply (intro global_conf_svrs_cls_twisted_update_cong, simp)
-      apply (intro fun_upd1_cong cl_conf.unfold_congs arg_cong[where f="(\<union>) _"], simp_all)
-      (* DOES NOT HOLD? (changes get_ts on server side) *)
-      sorry      
-    done
+  subgoal for s
+    by (auto simp add: tps_trans_defs)
+
+  subgoal for s
+    by (auto simp add: tps_trans_defs)
   done 
 
 \<comment> \<open>write_invoke\<close>
@@ -313,22 +267,13 @@ lemma write_invoke_write_invoke_indep:
 
 lemma write_invoke_write_commit_indep:
   "cl \<noteq> cl' \<Longrightarrow> left_commute tps (WInvoke cl kv_map) (WCommit cl' kv_map' cts' sn' u''')"
-  by (auto simp add: left_commute' tps_trans_defs fun_upd_twist)
+  apply (auto simp add: left_commute' tps_trans_defs fun_upd_twist)
+  (* SHOULD HOLD *)
+  sorry
 
 lemma write_invoke_write_done_indep:
   "cl \<noteq> cl' \<Longrightarrow> left_commute tps (WInvoke cl kv_map) (WDone cl' kv_map')"
-  apply (auto simp add: left_commute')
-  subgoal for s w s'
-  proof -
-    assume a: "cl \<noteq> cl'" "write_done cl' kv_map' s w" "write_invoke cl kv_map w s'"
-    hence "(\<lambda>ka. if kv_map' ka = None then lst_map (cls (write_invoke_U cl kv_map s) cl') ka
-              else get_lst (svr_state (svrs (write_invoke_U cl kv_map s) ka)
-                     (get_wtxn (write_invoke_U cl kv_map s) cl'))) = 
-           (\<lambda>k. if kv_map' k = None then lst_map (cls s cl') k
-              else get_lst (svr_state (svrs s k) (get_wtxn s cl')))" by auto
-    then show ?thesis using a by (auto simp add: tps_trans_defs fun_upd_twist)
-  qed
-  done
+  by (auto simp add: left_commute' tps_trans_defs fun_upd_twist ext)
 
 lemma write_invoke_register_read_indep:
   "cl \<noteq> get_cl t' \<Longrightarrow> left_commute tps (WInvoke cl kv_map) (RegR k' t' t_wr' rts')"
@@ -347,118 +292,145 @@ lemma write_invoke_commit_write_indep:
 
 lemma write_commit_read_invoke_indep:
   "cl \<noteq> cl' \<Longrightarrow> left_commute tps (WCommit cl kv_map cts sn u'') (RInvoke cl' keys')"
-  by (auto simp add: left_commute' tps_trans_defs fun_upd_twist)
+  apply (auto simp add: left_commute' tps_trans_top_defs)
+  subgoal for s
+    apply (auto simp add: tps_trans_GU_defs del: equalityI)
+    apply (intro arg_cong[where f="view_of _"])
+    (* UNCLEAR whether this holds, gst changes! *)
+    sorry
+
+  subgoal for s
+    by (simp_all add: tps_trans_GU_defs)
+
+  subgoal for s
+    by (auto simp add: tps_trans_GU_defs fun_upd_twist)
+  done
+
 
 lemma write_commit_read_indep:
   "cl \<noteq> cl' \<Longrightarrow> left_commute tps (WCommit cl kv_map cts sn u'') (Read cl' k' v' t' rts' rlst')"
-  by (auto simp add: left_commute' tps_trans_defs fun_upd_twist)
+  apply (auto simp add: left_commute' tps_trans_top_defs)
+  subgoal for s
+    apply (auto simp add: tps_trans_GU_defs)
+    apply (intro arg_cong[where f="view_of _"])
+    (* SHOULD HOLD *)
+    sorry
+
+  subgoal for s
+    by (simp_all add: tps_trans_GU_defs)
+
+  subgoal for s
+    by (auto simp add: tps_trans_GU_defs fun_upd_twist)
+  done
 
 lemma write_commit_read_done_indep:
   "cl \<noteq> cl' \<Longrightarrow> left_commute tps (WCommit cl kv_map cts sn u'') (RDone cl' kv_map' sn' u''')"
-  apply (auto simp add: left_commute' tps_trans_defs fun_upd_twist) oops
+  apply (auto simp add: left_commute' tps_trans_top_defs)
+  subgoal for s
+    apply (auto simp add: tps_trans_GU_defs)
+    apply (intro arg_cong[where f="view_of _"])
+    (* SHOULD HOLD *)
+    sorry
+
+  subgoal for s
+    apply (simp_all add: tps_trans_GU_defs)
+    sorry
+
+  subgoal for s
+    by (auto simp add: tps_trans_GU_defs fun_upd_twist)
+  done
 
 lemma write_commit_write_invoke_indep:
   "cl \<noteq> cl' \<Longrightarrow> left_commute tps (WCommit cl kv_map cts sn u'') (WInvoke cl' kv_map')"
-  by (auto simp add: left_commute' tps_trans_defs fun_upd_twist)
+  apply (auto simp add: left_commute' tps_trans_top_defs)
+  subgoal for s
+    apply (auto simp add: tps_trans_GU_defs)
+    apply (intro arg_cong[where f="view_of _"])
+    (* SHOULD HOLD *)
+    sorry
 
-lemma write_commit_write_commit_indep:
+  subgoal for s
+    by (simp_all add: tps_trans_GU_defs)
+
+  subgoal for s
+    by (auto simp add: tps_trans_GU_defs fun_upd_twist)
+  done
+
+
+lemma write_commit_write_commit_indep:    (* TRICKY?! *)
   "cl \<noteq> cl' \<Longrightarrow> left_commute tps (WCommit cl kv_map cts sn u'') (WCommit cl' kv_map' cts' sn' u''')"
-  by (auto simp add: left_commute' tps_trans_defs fun_upd_twist)
+  apply (auto simp add: left_commute' tps_trans_top_defs)
+  subgoal for s
+    apply (auto simp add: tps_trans_GU_defs)
+    
+    sorry
+
+  subgoal for s
+    apply (simp add: tps_trans_GU_defs)
+    sorry
+
+  subgoal for s
+    apply (auto simp add: tps_trans_GU_defs fun_upd_twist)
+    apply (intro global_conf.unfold_congs, simp_all)
+    apply auto
+    sorry
+  done
 
 lemma write_commit_write_done_indep:
   "cl \<noteq> cl' \<Longrightarrow> left_commute tps (WCommit cl kv_map cts sn u'') (WDone cl' kv_map')"
-  apply (auto simp add: left_commute')
-  subgoal for s w s'
-  proof -
-    assume a: "cl \<noteq> cl'" "write_done cl' kv_map' s w" "write_commit cl kv_map cts sn w s'"
-    hence "(\<lambda>ka. if kv_map' ka = None then lst_map (cls (write_commit_U cl kv_map cts s) cl') ka
-             else get_lst (svr_state (svrs (write_commit_U cl kv_map cts s) ka)
-                     (get_wtxn (write_commit_U cl kv_map cts s) cl'))) = 
-           (\<lambda>k. if kv_map' k = None then lst_map (cls s cl') k
-             else get_lst (svr_state (svrs s k) (get_wtxn s cl')))" 
-      by (auto simp add: write_commit_U_def)
-    then show ?thesis using a unfolding write_commit_U_def
-      by (auto simp add: tps_trans_defs fun_upd_twist)
-  qed
-  done
+  by (auto simp add: left_commute' tps_trans_defs fun_upd_twist get_view_def ext)
 
 lemma write_commit_register_read_indep:
   "cl \<noteq> get_cl t' \<Longrightarrow> left_commute tps (WCommit cl kv_map cts sn u'') (RegR k' t' t_wr' rts')"
-  apply (auto simp add: left_commute' write_commit_def register_read_def)
+  apply (auto simp add: left_commute' tps_trans_top_defs)
   subgoal for s
-    apply (simp add: write_commit_G_def register_read_U_def add_to_readerset_def
-        split: if_split_asm ver_state.split)
-    by (smt Collect_cong fun_upd_other fun_upd_same ver_state.distinct(5) ver_state.simps(10)
-        ver_state.simps(11) ver_state.simps(9))
-  by (simp_all add: register_read_G_def register_read_U_def write_commit_U_def)
+    apply (simp add: tps_trans_GU_defs add_to_readerset_def split: if_split_asm ver_state.split)
+    (* TBD *)
+    sorry
+  by (simp_all add: tps_trans_GU_defs)
 
 lemma write_commit_prepare_write_indep:
   "cl \<noteq> get_cl_w t' \<Longrightarrow> left_commute tps (WCommit cl kv_map cts sn u'') (PrepW k' t' v')"
-  apply (auto simp add: left_commute' write_commit_def prepare_write_def)
+  apply (auto simp add: left_commute' tps_trans_top_defs)
   subgoal for s
-    apply (auto simp add: write_commit_G_def prepare_write_U_def)
-    subgoal
-      by (smt (verit, best) domI fun_upd_apply option.simps(1) svr_conf.select_convs(1) 
-                svr_conf.simps(5) svr_conf.simps(6) svr_conf.simps(7) svr_conf.surjective)
-    subgoal
-      by metis
-    done
-  by (simp_all add: prepare_write_G_def prepare_write_U_def write_commit_U_def)
+    apply (auto simp add: tps_trans_GU_defs)
+    (* TBD *)
+    sorry
+  by (simp_all add: tps_trans_GU_defs)
 
 lemma write_commit_commit_write_indep:   
   "cl \<noteq> get_cl_w t' \<Longrightarrow> left_commute tps (WCommit cl kv_map cts sn u'') (CommitW k' t' v' cts')"
-  apply (auto simp add: left_commute' write_commit_def commit_write_def)
+  apply (auto simp add: left_commute' tps_trans_top_defs)
   subgoal for s
-    apply (auto simp add: write_commit_G_def commit_write_U_def)
-    subgoal
-      by (smt (verit, best) domI fun_upd_apply option.simps(1) svr_conf.select_convs(1) 
-                svr_conf.simps(5) svr_conf.simps(6) svr_conf.simps(7) svr_conf.surjective)
-    subgoal
-      by metis
-    done
-  by (simp_all add: commit_write_G_def commit_write_U_def write_commit_U_def)
-
+    apply (auto simp add: tps_trans_GU_defs)
+    (* TBD *)
+    sorry
+  subgoal for s
+    by (auto simp add: tps_trans_GU_defs)
+  subgoal for s
+    (* apply (simp add: tps_trans_GU_defs) *)      (* HANGS? *)
+    (* TBD *)
+    sorry
+  done
 
 \<comment> \<open>write_done\<close>
 
 lemma write_done_read_invoke_indep:
   "cl \<noteq> cl' \<Longrightarrow> left_commute tps (WDone cl kv_map) (RInvoke cl' keys')"
-  apply (auto simp add: left_commute')
-  subgoal for s w s'
-  proof -
-    assume a: "cl \<noteq> cl'" "read_invoke cl' keys' s w" "write_done cl kv_map w s'"
-    hence "(\<lambda>ka. if kv_map ka = None then lst_map (cls (read_invoke_U cl' keys' s) cl) ka
-             else get_lst (svr_state (svrs (read_invoke_U cl' keys' s) ka)
-                     (get_wtxn (read_invoke_U cl' keys' s) cl))) = 
-           (\<lambda>k. if kv_map k = None then lst_map (cls s cl) k
-             else get_lst (svr_state (svrs s k) (get_wtxn s cl)))" by auto
-    then show ?thesis using a by (auto simp add: tps_trans_defs fun_upd_twist)
-  qed
-  done
+  by (auto simp add: left_commute' tps_trans_defs fun_upd_twist ext)
 
 lemma write_done_read_indep:
   "cl \<noteq> cl' \<Longrightarrow> left_commute tps (WDone cl kv_map) (Read cl' k' v' t' rts' rlst')"
-  apply (auto simp add: left_commute')
-  subgoal for s w s'
-  proof -
-    assume a: "cl \<noteq> cl'" "read cl' k' v' t' rts' rlst' s w" "write_done cl kv_map w s'"
-    hence "(\<lambda>ka. if kv_map ka = None then lst_map (cls (read_U cl' k' v' rts' rlst' s) cl) ka
-             else get_lst (svr_state (svrs (read_U cl' k' v' rts' rlst' s) ka)
-                    (get_wtxn (read_U cl' k' v' rts' rlst' s) cl))) = 
-           (\<lambda>k. if kv_map k = None then lst_map (cls s cl) k
-             else get_lst (svr_state (svrs s k) (get_wtxn s cl)))" by auto
-    then show ?thesis using a by (auto simp add: tps_trans_defs fun_upd_twist)
-  qed
-  done
+  by (auto simp add: left_commute' tps_trans_defs fun_upd_twist ext)
 
 lemma write_done_read_done_indep:
   "cl \<noteq> cl' \<Longrightarrow> left_commute tps (WDone cl kv_map) (RDone cl' kv_map' sn' u''')"
-  apply (auto simp add: left_commute' read_done_def write_done_def)
+  apply (auto simp add: left_commute' tps_trans_top_defs)
   subgoal for s
-    by (auto simp add: tps_trans_defs)
+    by (auto simp add: tps_trans_GU_defs)
 
   subgoal for s
-    by (auto simp add: tps_trans_defs)
+    by (auto simp add: tps_trans_GU_defs get_view_def)
 
   subgoal for s
     apply (auto simp add: tps_trans_defs get_view_def global_conf_rtxn_cls_twisted_update_cong)
@@ -469,58 +441,15 @@ lemma write_done_read_done_indep:
 
 lemma write_done_write_invoke_indep:
   "cl \<noteq> cl' \<Longrightarrow> left_commute tps (WDone cl kv_map) (WInvoke cl' kv_map')"
-  apply (auto simp add: left_commute')
-  subgoal for s w s'
-  proof -
-    assume a: "cl \<noteq> cl'" "write_invoke cl' kv_map' s w" "write_done cl kv_map w s'"
-    hence "(\<lambda>ka. if kv_map ka = None then lst_map (cls (write_invoke_U cl' kv_map' s) cl) ka
-             else get_lst (svr_state (svrs (write_invoke_U cl' kv_map' s) ka)
-                    (get_wtxn (write_invoke_U cl' kv_map' s) cl))) = 
-           (\<lambda>k. if kv_map k = None then lst_map (cls s cl) k
-             else get_lst (svr_state (svrs s k) (get_wtxn s cl)))" by auto
-    then show ?thesis using a by (auto simp add: tps_trans_defs fun_upd_twist)
-  qed
-  done
+  by (auto simp add: left_commute' tps_trans_defs fun_upd_twist ext)
 
 lemma write_done_write_commit_indep:
   "cl \<noteq> cl' \<Longrightarrow> left_commute tps (WDone cl kv_map) (WCommit cl' kv_map' cts' sn' u''')"
-  apply (auto simp add: left_commute')
-  subgoal for s w s'
-  proof -
-    assume a: "cl \<noteq> cl'" "write_commit cl' kv_map' cts' sn' s w" "write_done cl kv_map w s'"
-    hence "(\<lambda>ka. if kv_map ka = None then lst_map (cls (write_commit_U cl' kv_map' cts' s) cl) ka
-             else get_lst (svr_state (svrs (write_commit_U cl' kv_map' cts' s) ka)
-                    (get_wtxn (write_commit_U cl' kv_map' cts' s) cl))) = 
-           (\<lambda>k. if kv_map k = None then lst_map (cls s cl) k
-             else get_lst (svr_state (svrs s k) (get_wtxn s cl)))" 
-      by (auto simp add: write_commit_U_def)
-    then show ?thesis using a unfolding write_commit_U_def
-      by (auto simp add: tps_trans_defs fun_upd_twist)
-  qed
-  done
+  by (auto simp add: left_commute' tps_trans_defs fun_upd_twist get_view_def ext)
 
 lemma write_done_write_done_indep:
   "cl \<noteq> cl' \<Longrightarrow> left_commute tps (WDone cl kv_map) (WDone cl' kv_map')"
-  apply (auto simp add: left_commute')
-  subgoal for s w s'
-  proof -
-    assume a: "cl \<noteq> cl'" "write_done cl' kv_map' s w" "write_done cl kv_map w s'"
-    hence wd1: "(\<lambda>ka. if kv_map ka = None then lst_map (cls (write_done_U cl' kv_map' s) cl) ka
-             else get_lst (svr_state (svrs (write_done_U cl' kv_map' s) ka)
-                    (get_wtxn (write_done_U cl' kv_map' s) cl))) = 
-           (\<lambda>k. if kv_map k = None then lst_map (cls s cl) k
-             else get_lst (svr_state (svrs s k) (get_wtxn s cl)))" 
-      by (auto simp add: write_done_U_def)
-    have "(\<lambda>ka. if kv_map' ka = None then lst_map (cls (write_done_U cl kv_map s) cl') ka
-             else get_lst (svr_state (svrs (write_done_U cl kv_map s) ka)
-                    (get_wtxn (write_done_U cl kv_map s) cl'))) = 
-           (\<lambda>k. if kv_map' k = None then lst_map (cls s cl') k
-             else get_lst (svr_state (svrs s k) (get_wtxn s cl')))" using a 
-      by (auto simp add: write_done_U_def)
-    then show ?thesis using a wd1 unfolding write_done_U_def
-      by (auto simp add: tps_trans_defs fun_upd_twist)
-  qed
-  done
+  by (auto simp add: left_commute'  tps_trans_defs fun_upd_twist ext)
 
 lemma write_done_server_ev_indep_L: 
   "{u.
@@ -571,18 +500,18 @@ lemmas write_done_register_read_indep_lemmas =
 
 lemma write_done_register_read_indep:
   "cl \<noteq> get_cl t' \<Longrightarrow> left_commute tps (WDone cl kv_map) (RegR k' t' t_wr' rts')"
-  apply (auto simp add: left_commute' write_done_def register_read_def)
+  apply (auto simp add: left_commute' tps_trans_top_defs)
   subgoal for s
-    apply (auto simp add: register_read_U_def write_done_G_def add_to_readerset_def
+    apply (auto simp add: tps_trans_GU_defs add_to_readerset_def
                 split: if_split_asm ver_state.split)
     by (smt  domI fun_upd_other fun_upd_same option.inject ver_state.case_eq_if ver_state.exhaust_sel
         ver_state.sel(2) ver_state.sel(4) ver_state.simps(10))
 
   subgoal for s
-    by (auto simp add: register_read_G_def write_done_U_def)
+    by (auto simp add: tps_trans_GU_defs)
 
   subgoal for s
-    apply (auto simp add: register_read_U_def write_done_U_def add_to_readerset_def
+    apply (auto simp add: tps_trans_GU_defs add_to_readerset_def
         write_done_register_read_indep_lemmas split: if_split_asm ver_state.split)
     done
   done
@@ -606,17 +535,17 @@ lemmas write_done_prepare_write_indep_lemmas =
 
 lemma write_done_prepare_write_indep:
   "cl \<noteq> get_cl_w t' \<Longrightarrow> left_commute tps (WDone cl kv_map) (PrepW k' t' v')"
-  apply (auto simp add: left_commute' write_done_def prepare_write_def)
+  apply (auto simp add: left_commute' tps_trans_top_defs)
   subgoal for s
-    apply (auto simp add: prepare_write_U_def write_done_G_def)
+    apply (auto simp add: tps_trans_GU_defs)
     by (smt (verit) domI fun_upd_apply get_cl_w.simps(2) option.sel svr_conf.select_convs(1) 
             svr_conf.simps(5) svr_conf.simps(6) svr_conf.simps(7) svr_conf.surjective)
 
   subgoal for s
-    by (auto simp add: prepare_write_G_def write_done_U_def)
+    by (auto simp add: tps_trans_GU_defs)
 
   subgoal for s
-    apply (auto simp add: prepare_write_U_def write_done_U_def write_done_prepare_write_indep_lemmas)
+    apply (auto simp add: tps_trans_GU_defs write_done_prepare_write_indep_lemmas)
     done
   done
 
@@ -641,18 +570,17 @@ lemmas write_done_commit_write_indep_lemmas =
 lemma write_done_commit_write_indep:  
   "\<lbrakk> cl \<noteq> get_cl_w t' \<rbrakk>
   \<Longrightarrow> left_commute tps (WDone cl kv_map) (CommitW k' t' v' cts')"
-  apply (auto simp add: left_commute' write_done_def commit_write_def)
+  apply (auto simp add: left_commute' tps_trans_top_defs)
   subgoal for s
-    apply (auto simp add: commit_write_U_def write_done_G_def)
+    apply (auto simp add: tps_trans_GU_defs)
     by (smt (verit) domI fun_upd_apply get_cl_w.simps(2) option.sel svr_conf.select_convs(1) 
             svr_conf.simps(5) svr_conf.simps(6) svr_conf.simps(7) svr_conf.surjective)
 
   subgoal for s
-    by (auto simp add: commit_write_G_def write_done_U_def)
+    by (auto simp add: tps_trans_GU_defs)
 
   subgoal for s
-    apply (auto simp add: commit_write_U_def write_done_U_def write_done_commit_write_indep_lemmas)
-    done
+    by (auto simp add: tps_trans_GU_defs write_done_commit_write_indep_lemmas)  (* SLOW *)
   done
 
 
@@ -668,18 +596,16 @@ lemma register_read_read_indep:
 
 lemma register_read_read_done_indep:
   "get_cl t \<noteq> cl' \<Longrightarrow> left_commute tps (RegR k t t_wr rts) (RDone cl' kv_map' sn' u''')"
-  apply (auto simp add: left_commute' read_done_def register_read_def)
+  apply (auto simp add: left_commute' tps_trans_top_defs )
   subgoal for s
-    by (auto simp add: tps_trans_defs)
+    by (auto simp add: tps_trans_GU_defs)
 
   subgoal for s
-    by (auto simp add: tps_trans_defs)
+    apply (auto simp add: tps_trans_GU_defs)
+    sorry
 
   subgoal for s
-    apply (auto simp add: tps_trans_defs get_view_def)
-    apply (intro global_conf_svrs_cls_twisted_update_cong[symmetric], simp)
-    apply (intro fun_upd1_cong cl_conf.fold_congs arg_cong[where f="(\<union>) _"], simp_all)
-    by (metis add_to_readerset_pres_read_at)
+    by (auto simp add: tps_trans_GU_defs)
   done 
 
 lemma register_read_write_invoke_indep:
@@ -688,27 +614,43 @@ lemma register_read_write_invoke_indep:
 
 lemma register_read_write_commit_indep:
   "get_cl t \<noteq> cl' \<Longrightarrow> left_commute tps (RegR k t t_wr rts) (WCommit cl' kv_map' cts' sn' u''')"
-  apply (auto simp add: left_commute' register_read_def write_commit_def)
-  apply (simp_all add: register_read_U_def register_read_G_def write_commit_G_def write_commit_U_def
-         add_to_readerset_def split: if_split_asm ver_state.split)
-  by (smt (verit) Collect_cong ver_state.distinct(5))
+  apply (auto simp add: left_commute' tps_trans_top_defs)
+  subgoal for s
+    by (simp_all add: tps_trans_GU_defs)
+
+  subgoal for s
+    apply (auto simp add: tps_trans_GU_defs)
+    subgoal for keys kv_map
+      (* TBD *)
+      sorry
+
+    subgoal for keys kv_map v
+      by (metis add_to_readerset_prep_inv domIff option.inject option.simps(3))
+
+    subgoal for keys kv_map
+      by (metis add_to_readerset_pres_get_ts)
+    done
+
+  subgoal for s
+    by (simp_all add: tps_trans_GU_defs)
+  done
+
 
 lemma register_read_write_done_indep:
   "get_cl t \<noteq> cl' \<Longrightarrow> left_commute tps (RegR k t t_wr rts) (WDone cl' kv_map')"
-  apply (auto simp add: left_commute' write_done_def register_read_def)
+  apply (auto simp add: left_commute' tps_trans_top_defs)
   subgoal for s
-    by (auto simp add: register_read_G_def write_done_U_def)
+    by (auto simp add: tps_trans_GU_defs)
 
   subgoal for s
-    apply (auto simp add: register_read_U_def write_done_G_def add_to_readerset_def
-                split: if_split_asm ver_state.split)
-    apply (metis domI ver_state.sel(2))
-    by (metis domIff option.discI option.sel ver_state.sel(4))
-
-  subgoal for s
-    apply (auto simp add: register_read_U_def write_done_U_def add_to_readerset_def
-        write_done_register_read_indep_lemmas split: if_split_asm ver_state.split)
+    apply (auto simp add: tps_trans_GU_defs add_to_readerset_def split: if_split_asm ver_state.split)
+    subgoal by (metis domI ver_state.sel(2))
+    subgoal by (metis domIff option.discI option.sel ver_state.sel(4))
     done
+
+  subgoal for s
+    by (auto simp add: tps_trans_GU_defs add_to_readerset_def write_done_register_read_indep_lemmas 
+             split: if_split_asm ver_state.split)
   done
 
 lemma register_read_register_read_indep:
@@ -736,7 +678,10 @@ lemma prepare_write_read_indep:
 
 lemma prepare_write_read_done_indep:
   "get_cl_w t \<noteq> cl' \<Longrightarrow> left_commute tps (PrepW k t v) (RDone cl' kv_map' sn' u''')"
-  apply (auto simp add: left_commute' tps_trans_defs fun_upd_twist) oops
+  apply (auto simp add: left_commute' tps_trans_defs fun_upd_twist) 
+  
+  
+  oops
 
 lemma prepare_write_write_invoke_indep:
   "get_cl_w t \<noteq> cl' \<Longrightarrow> left_commute tps (PrepW k t v) (WInvoke cl' kv_map')"
@@ -744,12 +689,17 @@ lemma prepare_write_write_invoke_indep:
 
 lemma prepare_write_write_commit_indep:
   "get_cl_w t \<noteq> cl' \<Longrightarrow> left_commute tps (PrepW k t v) (WCommit cl' kv_map' cts' sn' u''')"
-  apply (auto simp add: left_commute' prepare_write_def write_commit_def)
-  subgoal for s
-    by (auto simp add: prepare_write_G_def write_commit_U_def)
+  apply (auto simp add: left_commute' tps_trans_defs)
+  subgoal for s kvmap
+    apply (intro arg_cong[where f="view_of _"])
+    apply (simp add: get_view_def, intro ext)
+    apply (clarsimp simp add:  split: if_split)
+    (* DOES NOT SEEM TO HOLD :-/*)
+    sorry
 
-  apply (simp_all add: write_commit_G_def write_commit_U_def prepare_write_U_def)
-  by (smt (verit) Collect_cong get_cl_w.simps(2))
+  subgoal for s kvmap
+    by (smt (verit) Collect_cong get_cl_w.simps(2))
+  done
 
 lemma prepare_write_write_done_indep:
   "get_cl_w t \<noteq> cl' \<Longrightarrow> left_commute tps (PrepW k t v) (WDone cl' kv_map')"
@@ -790,20 +740,38 @@ lemma commit_write_write_invoke_indep:
 
 lemma commit_write_write_commit_indep:
   "get_cl_w t \<noteq> cl' \<Longrightarrow> left_commute tps (CommitW k t v cts) (WCommit cl' kv_map' cts' sn' u''')"
-  by (auto simp add: left_commute' tps_trans_defs) (metis)
+  apply (auto simp add: left_commute' tps_trans_top_defs) 
+  subgoal for s
+    by (auto simp add: tps_trans_GU_defs)
+
+  subgoal for s
+    apply (auto simp add: tps_trans_GU_defs)
+    (* TBD, 2 remaining subgoals *)
+    subgoal
+      apply (intro arg_cong[where f="view_of _"])
+      sorry
+    subgoal by metis
+    subgoal 
+      apply (intro arg_cong[where f="view_of _"])
+      sorry
+    subgoal by metis
+    sorry
+
+  subgoal for s
+    by (auto simp add: tps_trans_GU_defs)
+  done
 
 lemma commit_write_write_done_indep:
   "get_cl_w t \<noteq> cl' \<Longrightarrow> left_commute tps (CommitW k t v cts) (WDone cl' kv_map')"
-  apply (auto simp add: left_commute' write_done_def commit_write_def)
+  apply (auto simp add: left_commute' tps_trans_top_defs)
   subgoal for s
-    by (auto simp add: commit_write_G_def write_done_U_def)
+    by (auto simp add: tps_trans_GU_defs)
 
   subgoal for s
-    by (auto simp add: commit_write_U_def write_done_G_def)
+    by (auto simp add: tps_trans_GU_defs)
 
   subgoal for s 
-    apply (auto simp add: commit_write_U_def write_done_U_def write_done_commit_write_indep_lemmas)
-    done
+    by (auto simp add: tps_trans_GU_defs write_done_commit_write_indep_lemmas)  (* SLOW, ~15s *)
   done                                                                                                               
 
 lemma commit_write_register_read_indep:
